HOL/Order_Thms.thy
@@ -1,7 +1,7 @@
 (* Setup for proof steps related to ordering. *)
 
 theory Order_Thms
-imports Logic_Thms
+imports Logic_Thms HOL.Rat
 begin
 
 ML_file "util_arith.ML"
