ROOT
@@ -15,6 +15,8 @@ session AUTO2 = HOL_Base +
   description {*
     AUTO2 definitions.
   *}
+  sessions
+    "HOL_Base"
   theories
     "HOL/Auto2_Test"
     "HOL/Pelletier"
@@ -23,6 +25,8 @@ session Primes = AUTO2 +
   description {*
     Examples in number theory.
   *}
+  sessions
+    "AUTO2"
   theories
     "HOL/Primes_Ex"
 
@@ -30,6 +34,8 @@ session DataStrs_Basic = AUTO2 +
   description {*
     Functional data structures.
   *}
+  sessions
+    "AUTO2"
   theories
     "HOL/DataStrs/Arrays_Ex"
     "HOL/DataStrs/BST"
@@ -43,6 +49,8 @@ session DataStrs_Advanced = DataStrs_Basic +
   description {*
     Functional data structures, advanced.
   *}
+  sessions
+    "DataStrs_Basic"
   theories
     "HOL/DataStrs/Connectivity"
     "HOL/DataStrs/Dijkstra"
@@ -56,6 +64,8 @@ session DataStrs_FW = AUTO2 +
   description {*
     Floyd-Warshall algorithm.
   *}
+  sessions
+    "AUTO2"
   theories
     "HOL/DataStrs/Floyd_Warshall"
 
@@ -63,6 +73,8 @@ session SepLogic = DataStrs_Advanced +
   description {*
     Separation logic.
   *}
+  sessions
+    "DataStrs_Advanced"
   theories
     "HOL/SepLogic/Sep_Examples"
 
@@ -85,6 +97,8 @@ session FOL_Topology = Auto2_FOL +
   description {*
     Real numbers and topology in first order logic.
   *}
+  sessions
+    "Auto2_FOL"
   theories
     "FOL/Closure"
     "FOL/MetricSpaces"
@@ -93,6 +107,8 @@ session FOL_Homotopy = FOL_Topology +
   description {*
     Homotopy theory.
   *}
+  sessions
+    "FOL_Topology"
   theories
     "FOL/FundamentalGroup"
 
@@ -100,6 +116,8 @@ session FOL_Algebra = Auto2_FOL +
   description {*
     Abstract algebra.
   *}
+  sessions
+    "Auto2_FOL"
   theories
     "FOL/Module"
 
@@ -107,5 +125,7 @@ session FOL_Arrow = Auto2_FOL +
   description {*
     Arrow's theorem.
   *}
+  sessions
+    "Auto2_FOL"
   theories
     "FOL/ArrowImpossibility"
